theories/simple_sync.v
@@ -16,16 +16,14 @@ Definition mk_sync: val :=
           release "l";;
           "ret".
 
-Global Opaque mk_sync.
-
 Section syncer.
   Context `{!heapG Σ, !lockG Σ} (N: namespace).
   
-  Lemma mk_sync_spec: mk_syncer_spec N mk_sync.
+  Lemma mk_sync_spec: mk_syncer_spec mk_sync.
   Proof.
-    iIntros (R HN Φ) "(#Hh & HR) HΦ".
+    iIntros (R Φ) "HR HΦ".
     wp_seq. wp_bind (newlock _).
-    iApply (newlock_spec _ R with "[$Hh $HR]"); first done. iNext.
+    iApply (newlock_spec N R with "[HR]"); first done. iNext.
     iIntros (lk γ) "#Hl". wp_let. iApply "HΦ". iIntros "!#".
     iIntros (f). wp_let. iAlways.
     iIntros (P Q x) "#Hf !# HP".
